theories/logatom_stack/hocap_spec.v
@@ -1,0 +1,230 @@
+From stdpp Require Import namespaces.
+From iris.algebra Require Import excl auth list.
+From iris.heap_lang Require Export lifting notation.
+From iris.base_logic.lib Require Import invariants.
+From iris.program_logic Require Import atomic.
+From iris.heap_lang Require Import proofmode atomic_heap.
+From iris_examples.logatom_stack Require spec.
+Set Default Proof Using "Type".
+
+Module logatom := logatom_stack.spec.
+
+(** A general HoCAP-style interface for a stack, modeled after the spec in
+[hocap/abstract_bag.v].  There are two differences:
+- We split [bag_contents] into an authoritative part and a fragment as this
+  slightly strnegthens the spec: The logically atomic spec only requires
+  [stack_content ∗ stack_content] to derive a contradiction, the abstract bag
+  spec requires to get *three* pieces which is only possible when actually
+  calling a bag operation.
+- We also slightly weaken the spec by adding [make_laterable], which is needed
+  because logical atomicity can only capture laterable resources, which is
+  needed when implementing e.g. the elimination stack on top of an abstract
+  logically atomic heap. *)
+Record hocap_stack {Σ} `{!heapG Σ} := AtomicStack {
+  (* -- operations -- *)
+  new_stack : val;
+  push : val;
+  pop : val;
+  (* -- other data -- *)
+  name : Type;
+  (* -- predicates -- *)
+  is_stack (N : namespace) (γs : name) (v : val) : iProp Σ;
+  stack_content_frag (γs : name) (l : list val) : iProp Σ;
+  stack_content_auth (γs : name) (l : list val) : iProp Σ;
+  (* -- predicate properties -- *)
+  is_stack_persistent N γs v : Persistent (is_stack N γs v);
+  stack_content_frag_timeless γs l : Timeless (stack_content_frag γs l);
+  stack_content_auth_timeless γs l : Timeless (stack_content_auth γs l);
+  stack_content_frag_exclusive γs l1 l2 :
+    stack_content_frag γs l1 -∗ stack_content_frag γs l2 -∗ False;
+  stack_content_auth_exclusive γs l1 l2 :
+    stack_content_auth γs l1 -∗ stack_content_auth γs l2 -∗ False;
+  stack_content_agree γs l1 l2 :
+    stack_content_frag γs l1 -∗ stack_content_auth γs l2 -∗ ⌜l1 = l2⌝;
+  stack_content_update γs l l' :
+    stack_content_frag γs l -∗
+    stack_content_auth γs l -∗
+    |==> stack_content_frag γs l' ∗ stack_content_auth γs l';
+  (* -- operation specs -- *)
+  new_stack_spec N :
+    {{{ True }}} new_stack #() {{{ γs s, RET s; is_stack N γs s ∗ stack_content_frag γs [] }}};
+  push_spec N γs s e v (Φ : val → iProp Σ) :
+    IntoVal e v →
+    is_stack N γs s -∗
+    make_laterable (∀ l, stack_content_auth γs l ={⊤∖↑N}=∗ stack_content_auth γs (v::l) ∗ Φ #()) -∗
+    WP push (s, e) {{ Φ }};
+  pop_spec N γs s (Φ : val → iProp Σ) :
+    is_stack N γs s -∗
+    make_laterable (∀ l, stack_content_auth γs l ={⊤∖↑N}=∗
+          match l with [] => stack_content_auth γs [] ∗ Φ NONEV
+                | v :: l' => stack_content_auth γs l' ∗ Φ (SOMEV v) end) -∗
+    WP pop s {{ Φ }};
+}.
+Arguments hocap_stack _ {_}.
+
+Existing Instance is_stack_persistent.
+Existing Instance stack_content_frag_timeless.
+Existing Instance stack_content_auth_timeless.
+
+(** Show that our way of writing the [pop_spec] is equivalent to what is done in
+[concurrent_stack.spec].  IOW, the conjunction-vs-match doesn't matter.  Fixing
+the postcondition (the [Q] in [concurrent_stack.spec]) still matters. *)
+Section pop_equiv.
+  Context `{invG Σ} (T : Type).
+
+  Lemma pop_equiv E (I : list T → iProp Σ) (Φemp : iProp Σ) (Φret : T → iProp Σ) :
+    (∀ l, I l ={E}=∗
+       match l with [] => I [] ∗ Φemp | v :: l' => I l' ∗ Φret v end)
+    ⊣⊢
+    (∀ v vs, I (v :: vs) ={E}=∗ Φret v ∗ I vs)
+    ∧ (I [] ={E}=∗ Φemp ∗ I []).
+  Proof.
+    iSplit.
+    - iIntros "HΦ". iSplit.
+      + iIntros (??) "HI". iMod ("HΦ" with "HI") as "[$ $]". done.
+      + iIntros "HI". iMod ("HΦ" with "HI") as "[$ $]". done.
+    - iIntros "HΦ" (l) "HI". destruct l; rewrite [(I _ ∗ _)%I]bi.sep_comm; by iApply "HΦ".
+  Qed.
+End pop_equiv.
+
+(** From a HoCAP stack we can directly implement the logically atomic
+interface. *)
+Section hocap_logatom.
+  Context `{!heapG Σ} (stack: hocap_stack Σ).
+
+  Lemma logatom_push N γs s e v :
+    IntoVal e v →
+    stack.(is_stack) N γs s -∗
+    <<< ∀ l : list val, stack.(stack_content_frag) γs l >>>
+      stack.(push) (s, e) @ ⊤∖↑N
+    <<< stack.(stack_content_frag) γs (v::l), RET #() >>>.
+  Proof.
+    iIntros (?) "Hstack". iApply wp_atomic_intro. iIntros (Φ) "HΦ".
+    iApply (push_spec with "Hstack").
+    iApply (make_laterable_intro with "[%] [] HΦ"). iIntros "!# >HΦ" (l) "Hauth".
+    iMod "HΦ" as (l') "[Hfrag [_ Hclose]]".
+    iDestruct (stack_content_agree with "Hfrag Hauth") as %->.
+    iMod (stack_content_update with "Hfrag Hauth") as "[Hfrag $]".
+    iMod ("Hclose" with "Hfrag") as "HΦ". done.
+  Qed.
+
+  Lemma logatom_pop N γs (s : val) :
+    stack.(is_stack) N γs s -∗
+    <<< ∀ l : list val, stack.(stack_content_frag) γs l >>>
+      stack.(pop) s @ ⊤∖↑N
+    <<< stack.(stack_content_frag) γs (tail l),
+        RET match l with [] => NONEV | v :: _ => SOMEV v end >>>.
+  Proof.
+    iIntros "Hstack". iApply wp_atomic_intro. iIntros (Φ) "HΦ".
+    iApply (pop_spec with "Hstack").
+    iApply (make_laterable_intro with "[%] [] HΦ"). iIntros "!# >HΦ" (l) "Hauth".
+    iMod "HΦ" as (l') "[Hfrag [_ Hclose]]".
+    iDestruct (stack_content_agree with "Hfrag Hauth") as %->.
+    destruct l;
+    iMod (stack_content_update with "Hfrag Hauth") as "[Hfrag $]";
+    iMod ("Hclose" with "Hfrag") as "HΦ"; done.
+  Qed.
+
+  Definition hocap_logatom : logatom.atomic_stack Σ :=
+    {| logatom.new_stack_spec := stack.(new_stack_spec);
+       logatom.push_spec := logatom_push;
+       logatom.pop_spec := logatom_pop;
+       logatom.stack_content_exclusive := stack.(stack_content_frag_exclusive) |}.
+
+End hocap_logatom.
+
+(** From a logically atomic stack, we can implement a HoCAP stack by adding an
+auth invariant. *)
+
+(** The CMRA & functor we need. *)
+Class hocapG Σ := HocapG {
+  hocap_stateG :> inG Σ (authR (optionUR $ exclR (listC valC)));
+}.
+Definition hocapΣ : gFunctors :=
+  #[GFunctor (exclR unitC); GFunctor (authR (optionUR $ exclR (listC valC)))].
+
+Instance subG_hocapΣ {Σ} : subG hocapΣ Σ → hocapG Σ.
+Proof. solve_inG. Qed.
+
+Section logatom_hocap.
+  Context `{!heapG Σ} `{!hocapG Σ} (stack: logatom.atomic_stack Σ).
+
+  Definition hocap_name : Type := stack.(logatom.name) * gname.
+  Implicit Types γs : hocap_name.
+
+  Definition hocap_stack_content_auth γs l : iProp Σ := own γs.2 (● Excl' l).
+  Definition hocap_stack_content_frag γs l : iProp Σ := own γs.2 (◯ Excl' l).
+
+  Definition hocap_is_stack N γs v : iProp Σ :=
+    (stack.(logatom.is_stack) (N .@ "stack") γs.1 v ∗
+     inv (N .@ "wrapper") (∃ l, stack.(logatom.stack_content) γs.1 l ∗ hocap_stack_content_auth γs l))%I.
+
+  Lemma hocap_new_stack N :
+    {{{ True }}}
+      stack.(logatom.new_stack) #()
+    {{{ γs s, RET s; hocap_is_stack N γs s ∗ hocap_stack_content_frag γs [] }}}.
+  Proof.
+    iIntros (Φ) "_ HΦ". iApply wp_fupd. iApply logatom.new_stack_spec; first done.
+    iIntros "!>" (γs s) "[Hstack Hcont]".
+    iMod (own_alloc (● Excl' [] ⋅ ◯ Excl' [])) as (γw) "[Hs● Hs◯]".
+    { apply auth_valid_discrete_2. split; done. }
+    iApply ("HΦ" $! (γs, γw)). rewrite /hocap_is_stack. iFrame.
+    iApply inv_alloc. eauto with iFrame.
+  Qed.
+
+  Lemma hocap_push N γs s e v (Φ : val → iProp Σ) :
+    IntoVal e v →
+    hocap_is_stack N γs s -∗
+    make_laterable (∀ l, hocap_stack_content_auth γs l ={⊤∖↑N}=∗ hocap_stack_content_auth γs (v::l) ∗ Φ #()) -∗
+    WP stack.(logatom.push) (s, e) {{ Φ }}.
+  Proof using Type*.
+    iIntros (?) "#[Hstack Hwrap] Hupd". iApply (logatom.push_spec with "Hstack"); first iAccu.
+    iAuIntro. iInv "Hwrap" as (l) "[>Hcont >H●]".
+    iAaccIntro with "Hcont"; first by eauto 10 with iFrame.
+    iIntros "Hcont".
+    iMod fupd_intro_mask' as "Hclose";
+      last iMod (make_laterable_elim with "Hupd H●") as "[H● HΦ]"; first solve_ndisj.
+    iMod "Hclose" as "_". iIntros "!>".
+    eauto with iFrame.
+  Qed.
+
+  Lemma hocap_pop N γs s (Φ : val → iProp Σ) :
+    hocap_is_stack N γs s -∗
+    make_laterable (∀ l, hocap_stack_content_auth γs l ={⊤∖↑N}=∗
+          match l with [] => hocap_stack_content_auth γs [] ∗ Φ NONEV
+                | v :: l' => hocap_stack_content_auth γs l' ∗ Φ (SOMEV v) end) -∗
+    WP stack.(logatom.pop) s {{ Φ }}.
+  Proof using Type*.
+    iIntros "#[Hstack Hwrap] Hupd". iApply (logatom.pop_spec with "Hstack"); first iAccu.
+    iAuIntro. iInv "Hwrap" as (l) "[>Hcont >H●]".
+    iAaccIntro with "Hcont"; first by eauto 10 with iFrame.
+    iIntros "Hcont". destruct l.
+    - iMod fupd_intro_mask' as "Hclose";
+        last iMod (make_laterable_elim with "Hupd H●") as "[H● HΦ]"; first solve_ndisj.
+       iMod "Hclose" as "_". iIntros "!>"; eauto with iFrame.
+    - iMod fupd_intro_mask' as "Hclose";
+        last iMod (make_laterable_elim with "Hupd H●") as "[H● HΦ]"; first solve_ndisj.
+       iMod "Hclose" as "_". iIntros "!>"; eauto with iFrame.
+  Qed.
+
+  Program Definition logatom_hocap : hocap_stack Σ :=
+    {| new_stack_spec := hocap_new_stack;
+       push_spec := hocap_push;
+       pop_spec := hocap_pop |}.
+  Next Obligation.
+    iIntros (???) "Hf1 Hf2". iDestruct (own_valid_2 with "Hf1 Hf2") as %[].
+  Qed.
+  Next Obligation.
+    iIntros (???) "Ha1 Ha2". iDestruct (own_valid_2 with "Ha1 Ha2") as %[].
+  Qed.
+  Next Obligation.
+    iIntros (???) "Hf Ha". iDestruct (own_valid_2 with "Ha Hf") as
+      %[->%Excl_included%leibniz_equiv _]%auth_valid_discrete_2. done.
+  Qed.
+  Next Obligation.
+    iIntros (???) "Hf Ha". iMod (own_update_2 with "Ha Hf") as "[? ?]".
+    { eapply auth_update, option_local_update, (exclusive_local_update _ (Excl _)). done. }
+    by iFrame.
+  Qed.
+
+End logatom_hocap.
